Revert "regressions for `as` keyword"
This reverts commit e894b19be1694201c017b01f8522c0499012ee6e.

ulib/FStar.List.Tot.Properties.fst
@@ -343,9 +343,9 @@ let rec lemma_unsnoc_append (#a:Type) (l1 l2:list a) :
   Lemma
     (requires (length l2 > 0)) // the [length l2 = 0] is trivial
     (ensures (
-        let aa, a = unsnoc (l1 @ l2) in
-        let bb, b = unsnoc l2 in
-        aa == l1 @ bb /\ a == b)) =
+        let as, a = unsnoc (l1 @ l2) in
+        let bs, b = unsnoc l2 in
+        as == l1 @ bs /\ a == b)) =
   match l1 with
   | [] -> ()
   | _ :: l1' -> lemma_unsnoc_append l1' l2
@@ -381,11 +381,11 @@ let rec split_using (#t:Type) (l:list t) (x:t{x `memP` l}) :
   GTot (list t * list t) =
   match l with
   | [_] -> [], l
-  | a :: aa ->
+  | a :: as ->
     if FStar.StrongExcludedMiddle.strong_excluded_middle (a == x) then (
       [], l
     ) else (
-      let l1', l2' = split_using aa x in
+      let l1', l2' = split_using as x in
       a :: l1', l2'
     )
 
@@ -399,7 +399,7 @@ let rec lemma_split_using (#t:Type) (l:list t) (x:t{x `memP` l}) :
         append l1 l2 == l)) =
   match l with
   | [_] -> ()
-  | a :: aa ->
+  | a :: as ->
     let goal =
       let l1, l2 = split_using l x in
         length l2 > 0 /\
@@ -411,7 +411,7 @@ let rec lemma_split_using (#t:Type) (l:list t) (x:t{x `memP` l}) :
       #_ #_
       #(fun () -> goal)
       (fun (_:squash (a == x)) -> ())
-      (fun (_:squash (x `memP` aa)) -> lemma_split_using aa x)
+      (fun (_:squash (x `memP` as)) -> lemma_split_using as x)
 
 (** Definition of [index_of] *)
 
@@ -422,11 +422,11 @@ let rec index_of (#t:Type) (l:list t) (x:t{x `memP` l}) :
   GTot (i:nat{i < length l /\ index l i == x}) =
   match l with
   | [_] -> 0
-  | a :: aa ->
+  | a :: as ->
     if FStar.StrongExcludedMiddle.strong_excluded_middle (a == x) then (
       0
     ) else (
-      1 + index_of aa x
+      1 + index_of as x
     )
 
 (** Properties about partition **)
